Batteries/Data/Fin.lean
@@ -1,2 +1,4 @@
 import Batteries.Data.Fin.Basic
+import Batteries.Data.Fin.Coding
+import Batteries.Data.Fin.Enum
 import Batteries.Data.Fin.Lemmas
