Batteries/Data/Fin/Coding.lean
@@ -1,0 +1,497 @@
+/-
+Copyright (c) 2024 François G. Dorais. All rights reserved.
+Released under Apache 2.0 license as described in the file LICENSE.
+Authors: François G. Dorais
+-/
+import Batteries.Data.Fin.Lemmas
+import Batteries.Tactic.Basic
+import Batteries.Tactic.Trans
+import Batteries.Tactic.Lint
+
+namespace Fin
+
+/-- Encode a unit value as a `Fin` type. -/
+@[nolint unusedArguments]
+def encodePUnit : PUnit → Fin 1
+  | .unit => 0
+
+/-- Decode a unit value as a `Fin` type. -/
+@[pp_nodot] def decodePUnit : Fin 1 → PUnit
+  | 0 => .unit
+
+/-- Encode a unit value as a `Fin` type. -/
+abbrev encodeUnit : Unit → Fin 1 := encodePUnit
+
+/-- Decode a unit value as a `Fin` type. -/
+@[pp_nodot] abbrev decodeUnit : Fin 1 → Unit := decodePUnit
+
+@[simp] theorem encodePUnit_decodePUnit : (x : Fin 1) → encodePUnit (decodePUnit x) = x
+  | 0 => rfl
+
+@[simp] theorem decodePUnit_encodePUnit : (x : PUnit) → decodePUnit (encodePUnit x) = x
+  | .unit => rfl
+
+/-- Encode a boolean value as a `Fin` type. -/
+def encodeBool : Bool → Fin 2
+  | false => 0
+  | true => 1
+
+/-- Decode a boolean value as a `Fin` type. -/
+@[pp_nodot] def decodeBool : Fin 2 → Bool
+  | 0 => false
+  | 1 => true
+
+@[simp] theorem encodeBool_decodeBool : (x : Fin 2) → encodeBool (decodeBool x) = x
+  | 0 => rfl
+  | 1 => rfl
+
+@[simp] theorem decodeBool_encodeBool : (x : Bool) → decodeBool (encodeBool x) = x
+  | false => rfl
+  | true => rfl
+
+/-- Decode an optional `Fin` types. -/
+def encodeOption : Option (Fin n) → Fin (n+1)
+  | none => 0
+  | some x => x.succ
+
+/-- Decode an optional `Fin` types. -/
+@[pp_nodot] def decodeOption (x : Fin (n+1)) : Option (Fin n) :=
+  if h : x = 0 then
+    none
+  else
+    some (x.pred h)
+
+@[simp] theorem encodeOption_decodeOption (x : Fin (n+1)) : encodeOption (decodeOption x) = x := by
+  simp only [encodeOption, decodeOption]
+  split
+  · next hd =>
+    split at hd
+    · next he => cases he; rfl
+    · contradiction
+  · next hd =>
+    split at hd
+    · contradiction
+    · next he => cases hd; simp
+
+@[simp] theorem decodeOption_encodeOption (x : Option (Fin n)) :
+    decodeOption (encodeOption x) = x := by
+  simp only [encodeOption, decodeOption]
+  split
+  · next he =>
+    split at he
+    · rfl
+    · simp only [Fin.succ] at he; cases he
+  · next he =>
+    split at he
+    · simp at he
+    · rfl
+
+/-- Encode a sum of `Fin` types. -/
+def encodeSum : Sum (Fin n) (Fin m) → Fin (n + m)
+  | .inl x => x.castLE (Nat.le_add_right _ _)
+  | .inr x => x.natAdd n
+
+/-- Decode a sum of `Fin` types. -/
+@[pp_nodot] def decodeSum (x : Fin (n + m)) : Sum (Fin n) (Fin m) :=
+  if h : x < n then
+    .inl ⟨x, h⟩
+  else
+    .inr ⟨x - n, by omega⟩
+
+@[simp] theorem encodeSum_decodeSum (x : Fin (n + m)) : encodeSum (decodeSum x) = x := by
+  simp only [encodeSum, decodeSum]
+  split
+  · next hd =>
+    split at hd
+    · cases hd; rfl
+    · contradiction
+  · next hd =>
+    split at hd
+    · contradiction
+    · next he =>
+      cases x; cases hd
+      simp at he ⊢; omega
+
+@[simp] theorem decodeSum_encodeSum (x : Sum (Fin n) (Fin m)) : decodeSum (encodeSum x) = x := by
+  simp only [encodeSum, decodeSum]
+  split
+  · next hd =>
+    split
+    · simp
+    · simp at hd; omega
+  · next hd =>
+    split
+    · simp at hd
+    · next x =>
+      cases x
+      simp; omega
+
+/-- Encode a product of `Fin` types. -/
+def encodeProd : Fin m × Fin n → Fin (m * n)
+  | (⟨i, hi⟩, ⟨j, hj⟩) => Fin.mk (n * i + j) <| calc
+    _ < n * i + n := Nat.add_lt_add_left hj ..
+    _ = n * (i + 1) := Nat.mul_succ ..
+    _ ≤ n * m := Nat.mul_le_mul_left n (Nat.succ_le_of_lt hi)
+    _ = m * n := Nat.mul_comm ..
+
+/-- Decode a product of `Fin` types. -/
+@[pp_nodot] def decodeProd (z : Fin (m * n)) : Fin m × Fin n :=
+  ⟨left, right⟩
+where
+  hn : 0 < n := by
+    apply Nat.zero_lt_of_ne_zero
+    intro h
+    absurd z.is_lt
+    simp [h]
+  /-- Left case of `decodeProd`. -/
+  left := ⟨z / n, by rw [Nat.div_lt_iff_lt_mul hn]; exact z.is_lt⟩
+  /-- Right case of `decodeProd`. -/
+  right := ⟨z % n, Nat.mod_lt _ hn⟩
+
+@[simp] theorem encodeProd_decodeProd (x : Fin (m * n)) : encodeProd (decodeProd x) = x := by
+  simp [encodeProd, decodeProd, decodeProd.left, decodeProd.right, Nat.div_add_mod]
+
+@[simp] theorem decodeProd_encodeProd (x : Fin m × Fin n) : decodeProd (encodeProd x) = x := by
+  match x with
+  | ⟨⟨_, _⟩, ⟨_, h⟩⟩ => simp [encodeProd, decodeProd, decodeProd.left, decodeProd.right,
+    Nat.mul_add_div (Nat.zero_lt_of_lt h), Nat.div_eq_of_lt h, Nat.mul_add_mod, Nat.mod_eq_of_lt h]
+
+/-- Encode a dependent sum of `Fin` types. -/
+def encodeSigma (f : Fin n → Nat) (x : (i : Fin n) × Fin (f i)) : Fin (Fin.sum f) :=
+  match n, f, x with
+  | _+1, _, ⟨⟨0, _⟩, ⟨j, hj⟩⟩ =>
+    ⟨j, Nat.lt_of_lt_of_le hj (sum_succ .. ▸ Nat.le_add_right ..)⟩
+  | _+1, f, ⟨⟨i+1, hi⟩, ⟨j, hj⟩⟩ =>
+    match encodeSigma ((f ∘ succ)) ⟨⟨i, Nat.lt_of_succ_lt_succ hi⟩, ⟨j, hj⟩⟩ with
+    | ⟨k, hk⟩ => ⟨f 0 + k, sum_succ .. ▸ Nat.add_lt_add_left hk ..⟩
+
+/-- Decode a dependent sum of `Fin` types. -/
+@[pp_nodot] def decodeSigma (f : Fin n → Nat) (x : Fin (Fin.sum f)) : (i : Fin n) × Fin (f i) :=
+  match n, f, x with
+  | 0, _, ⟨_, h⟩ => False.elim (by simp at h)
+  | n+1, f, ⟨x, hx⟩ =>
+    if hx0 : x < f 0 then
+      ⟨0, ⟨x, hx0⟩⟩
+    else
+      have hxf : x - f 0 < Fin.sum (f ∘ succ) := by
+        apply Nat.sub_lt_left_of_lt_add
+        · exact Nat.le_of_not_gt hx0
+        · rw [← sum_succ]; exact hx
+      match decodeSigma ((f ∘ succ)) ⟨x - f 0, hxf⟩ with
+      | ⟨⟨i, hi⟩, y⟩ => ⟨⟨i+1, Nat.succ_lt_succ hi⟩, y⟩
+
+@[simp] theorem encodeSigma_decodeSigma (f : Fin n → Nat) (x : Fin (Fin.sum f)) :
+    encodeSigma f (decodeSigma f x) = x := by
+  induction n with
+  | zero => absurd x.is_lt; simp
+  | succ n ih =>
+    simp only [decodeSigma]
+    split
+    · simp [encodeSigma]
+    · next h1 =>
+      have h2 : x - f 0 < Fin.sum (f ∘ succ) := by
+        apply Nat.sub_lt_left_of_lt_add
+        · exact Nat.le_of_not_gt h1
+        · rw [← sum_succ]; exact x.is_lt
+      have : encodeSigma (f ∘ succ) (decodeSigma (f ∘ succ) ⟨x - f 0, h2⟩) = ↑x - f 0 := by
+        rw [ih]
+      ext; simp only [encodeSigma]
+      conv => rhs; rw [← Nat.add_sub_of_le (Nat.le_of_not_gt h1)]
+      congr
+
+@[simp] theorem decodeSigma_encodeSigma (f : Fin n → Nat) (x : (i : Fin n) × Fin (f i)) :
+    decodeSigma f (encodeSigma f x) = x := by
+  induction n with
+  | zero => nomatch x
+  | succ n ih =>
+    simp only [decodeSigma]
+    match x with
+    | ⟨0, x⟩ => simp [encodeSigma]
+    | ⟨⟨i+1, hi⟩, ⟨x, hx⟩⟩ =>
+      have : ¬ encodeSigma f ⟨⟨i+1, hi⟩, ⟨x, hx⟩⟩ < f 0 := by simp [encodeSigma]
+      rw [dif_neg this]
+      have : (encodeSigma f ⟨⟨i+1, hi⟩, ⟨x, hx⟩⟩).1 - f 0 =
+          (encodeSigma (f ∘ Fin.succ) ⟨⟨i, Nat.lt_of_succ_lt_succ hi⟩, ⟨x, hx⟩⟩).1 := by
+        simp [encodeSigma, Nat.add_sub_cancel_left]
+      have h := ih (f ∘ Fin.succ) ⟨⟨i, Nat.lt_of_succ_lt_succ hi⟩, ⟨x, hx⟩⟩
+      simp [Sigma.ext_iff, Fin.ext_iff] at h ⊢
+      constructor
+      · conv => rhs; rw [← h.1]
+        apply congrArg
+        apply congrArg Sigma.fst
+        congr
+      · apply HEq.trans _ h.2; congr
+
+/-- Encode a function between `Fin` types. -/
+def encodeFun : {m : Nat} → (Fin m → Fin n) → Fin (n ^ m)
+  | 0, _ => ⟨0, by simp⟩
+  | m+1, f => Fin.mk (n * (encodeFun fun k => f k.succ).val + (f 0).val) <| calc
+    _ < n * (encodeFun fun k => f k.succ).val + n := Nat.add_lt_add_left (f 0).isLt _
+    _ = n * ((encodeFun fun k => f k.succ).val + 1) := Nat.mul_succ ..
+    _ ≤ n * n ^ m := Nat.mul_le_mul_left n (Nat.succ_le_of_lt (encodeFun fun k => f k.succ).isLt)
+    _ = n ^ m * n := Nat.mul_comm ..
+    _ = n ^ (m+1) := Nat.pow_succ ..
+
+/-- Decode a function between `Fin` types. -/
+@[pp_nodot] def decodeFun : {m : Nat} → Fin (n ^ m) → Fin m → Fin n
+  | 0, _ => (nomatch .)
+  | m+1, ⟨k, hk⟩ =>
+    have hn : n > 0 := by
+      apply Nat.zero_lt_of_ne_zero
+      intro h
+      rw [h, Nat.pow_succ, Nat.mul_zero] at hk
+      contradiction
+    fun
+    | 0 => ⟨k % n, Nat.mod_lt k hn⟩
+    | ⟨i+1, hi⟩ =>
+      have h : k / n < n ^ m := by rw [Nat.div_lt_iff_lt_mul hn]; exact hk
+      decodeFun ⟨k / n, h⟩ ⟨i, Nat.lt_of_succ_lt_succ hi⟩
+
+@[simp] theorem encodeFun_decodeFun (x : Fin (n ^ m)) : encodeFun (decodeFun x) = x := by
+  induction m with simp only [encodeFun, decodeFun, Fin.succ]
+  | zero => simp; omega
+  | succ m ih => cases x; simp [ih]; rw [← Fin.zero_eta, Nat.div_add_mod]
+
+@[simp] theorem decodeFun_encodeFun (x : Fin m → Fin n) : decodeFun (encodeFun x) = x := by
+  funext i; induction m with simp only [encodeFun, decodeFun]
+  | zero => nomatch i
+  | succ m ih =>
+    have hn : 0 < n := Nat.zero_lt_of_lt (x 0).is_lt
+    split
+    · ext; simp [Nat.mul_add_mod, Nat.mod_eq_of_lt]
+    · next i hi =>
+      have : decodeFun (encodeFun fun k => x k.succ) ⟨i, Nat.lt_of_succ_lt_succ hi⟩
+          = x ⟨i+1, hi⟩ := by rw [ih]; rfl
+      simp [← this, Nat.mul_add_div hn, Nat.div_eq_of_lt]
+
+/-- Encode a dependent product of `Fin` types. -/
+def encodePi (f : Fin n → Nat) (x : (i : Fin n) → Fin (f i)) : Fin (Fin.prod f) :=
+  match n, f, x with
+  | 0, _, _ => ⟨0, by simp [Fin.prod]⟩
+  | _+1, f, x =>
+    match encodePi ((f ∘ succ)) (fun ⟨i, hi⟩ => x ⟨i+1, Nat.succ_lt_succ hi⟩) with
+    | ⟨k, hk⟩ => Fin.mk (f 0 * k + (x 0).val) $ calc
+      _ < f 0 * k + f 0 := Nat.add_lt_add_left (x 0).isLt ..
+      _ = f 0 * (k + 1) := Nat.mul_succ ..
+      _ ≤ f 0 * Fin.prod (f ∘ succ) := Nat.mul_le_mul_left _ (Nat.succ_le_of_lt hk)
+      _ = Fin.prod f := Eq.symm <| prod_succ ..
+
+/-- Decode a dependent product of `Fin` types. -/
+def decodePi (f : Fin n → Nat) (x : Fin (Fin.prod f)) : (i : Fin n) → Fin (f i) :=
+  match n, f, x with
+  | 0, _, _ => (nomatch ·)
+  | n+1, f, ⟨x, hx⟩ =>
+    have h : f 0 > 0 := by
+      apply Nat.zero_lt_of_ne_zero
+      intro h
+      rw [prod_succ, h, Nat.zero_mul] at hx
+      contradiction
+    have : x / f 0 < Fin.prod (f ∘ succ) := by
+      rw [Nat.div_lt_iff_lt_mul h, Nat.mul_comm, ← prod_succ]
+      exact hx
+    match decodePi ((f ∘ succ)) ⟨x / f 0, this⟩ with
+    | t => fun
+      | ⟨0, _⟩ => ⟨x % f 0, Nat.mod_lt x h⟩
+      | ⟨i+1, hi⟩ => t ⟨i, Nat.lt_of_succ_lt_succ hi⟩
+
+@[simp] theorem encodePi_decodePi (f : Fin n → Nat) (x : Fin (Fin.prod f)) :
+    encodePi f (decodePi f x) = x := by
+  induction n with
+  | zero =>
+    match x with
+    | ⟨0, _⟩ => rfl
+    | ⟨_+1, h⟩ => simp at h
+  | succ n ih =>
+    simp only [encodePi, decodePi, ih]
+    ext
+    conv => rhs; rw [← Nat.div_add_mod x (f 0)]
+    congr
+
+@[simp] theorem decodePi_encodePi (f : Fin n → Nat) (x : (i : Fin n) → Fin (f i)) :
+    decodePi f (encodePi f x) = x := by
+  induction n with
+  | zero => funext i; nomatch i
+  | succ n ih =>
+    have h0 : 0 < f 0 := Nat.zero_lt_of_lt (x 0).is_lt
+    funext i
+    simp only [decodePi]
+    split
+    · simp [Nat.mul_add_mod, Nat.mod_eq_of_lt (x 0).is_lt]
+    · next i hi =>
+      have h : decodePi (f ∘ succ) (encodePi (f ∘ succ) fun i => x i.succ)
+          ⟨i, Nat.lt_of_succ_lt_succ hi⟩ = x ⟨i+1, hi⟩ := by rw [ih]; rfl
+      conv => rhs; rw [← h]
+      congr; simp [Nat.mul_add_div h0, Nat.div_eq_of_lt (x 0).is_lt]; rfl
+
+/-- Encode a decidable subtype of a `Fin` type. -/
+def encodeSubtype (P : Fin n → Prop) [inst : DecidablePred P] (i : { i // P i }) :
+    Fin (Fin.count P) :=
+  match n, P, inst, i with
+  | n+1, P, inst, ⟨0, hp⟩ =>
+    have : Fin.count P > 0 := by simp [count_succ, hp]
+    ⟨0, this⟩
+  | n+1, P, inst, ⟨⟨i+1, hi⟩, hp⟩ =>
+    match encodeSubtype (fun i => P i.succ) ⟨⟨i, Nat.lt_of_succ_lt_succ hi⟩, hp⟩ with
+    | ⟨k, hk⟩ =>
+      if h0 : P 0 then
+        have : Fin.count P = (Fin.count fun i => P i.succ) + 1 := by
+          simp_arith only [count_succ, Function.comp_def, if_pos h0]
+        this ▸ ⟨k+1, Nat.succ_lt_succ hk⟩
+      else
+        have : Fin.count P = Fin.count fun i => P i.succ := by simp [count_succ, h0]
+        this ▸ ⟨k, hk⟩
+
+/-- Decode a decidable subtype of a `Fin` type. -/
+def decodeSubtype (p : Fin n → Prop) [inst : DecidablePred p] (k : Fin (Fin.count p)) :
+    { i // p i } :=
+  match n, p, inst, k with
+  | 0, _, _, ⟨_, h⟩ => False.elim (by simp at h)
+  | n+1, p, inst, ⟨k, hk⟩ =>
+    if h0 : p 0 then
+      have : Fin.count p = (Fin.count fun i => p i.succ) + 1 := by simp [count_succ, h0]
+      match k with
+      | 0 => ⟨0, h0⟩
+      | k + 1 =>
+        match decodeSubtype (fun i => p i.succ) ⟨k, Nat.lt_of_add_lt_add_right (this ▸ hk)⟩ with
+        | ⟨⟨i, hi⟩, hp⟩ => ⟨⟨i+1, Nat.succ_lt_succ hi⟩, hp⟩
+    else
+      have : Fin.count p = Fin.count fun i => p i.succ := by simp [count_succ, h0]
+      match decodeSubtype (fun i => p (succ i)) ⟨k, this ▸ hk⟩ with
+      | ⟨⟨i, hi⟩, hp⟩ => ⟨⟨i+1, Nat.succ_lt_succ hi⟩, hp⟩
+
+@[simp] theorem encodeSubtype_decodeSubtype (P : Fin n → Prop) [DecidablePred P]
+    (x : Fin (Fin.count P)) : encodeSubtype P (decodeSubtype P x) = x := by
+  induction n with
+  | zero => absurd x.is_lt; simp
+  | succ n ih =>
+    simp only [decodeSubtype]
+    split
+    · ext; split <;> simp [encodeSubtype, count_succ, *]
+    · ext; simp [encodeSubtype, count_succ, *]
+
+theorem encodeSubtype_zero_pos {P : Fin (n+1) → Prop} [DecidablePred P] (h₀ : P 0) :
+    encodeSubtype P ⟨0, h₀⟩ = ⟨0, by simp [count_succ, *]⟩ := by
+  ext; simp [encodeSubtype]
+
+theorem encodeSubtype_succ_pos {P : Fin (n+1) → Prop} [DecidablePred P] (h₀ : P 0) {i : Fin n}
+    (h : P i.succ) : encodeSubtype P ⟨i.succ, h⟩ =
+      (encodeSubtype (fun i => P i.succ) ⟨i, h⟩).succ.cast (by simp [count_succ, *]) := by
+  ext; simp [encodeSubtype, count_succ, *]
+
+theorem encodeSubtype_succ_neg {P : Fin (n+1) → Prop} [DecidablePred P] (h₀ : ¬ P 0) {i : Fin n}
+    (h : P i.succ) : encodeSubtype P ⟨i.succ, h⟩ =
+      (encodeSubtype (fun i => P i.succ) ⟨i, h⟩).cast (by simp [count_succ, *]) := by
+  ext; simp [encodeSubtype, count_succ, *]
+
+@[simp] theorem decodeSubtype_encodeSubtype (P : Fin n → Prop) [DecidablePred P] (x : { x // P x}) :
+    decodeSubtype P (encodeSubtype P x) = x := by
+  match x with
+  | ⟨i, h⟩ =>
+    induction n with
+    | zero => absurd x.val.is_lt; simp
+    | succ n ih =>
+      if h₀ : P 0 then
+        simp only [decodeSubtype, dif_pos h₀]
+        cases i using Fin.casesZeroSuccOn with
+        | zero => rw [encodeSubtype_zero_pos h₀]
+        | succ i =>
+          rw [encodeSubtype_succ_pos h₀]
+          simp only [coe_cast, val_succ, Subtype.mk.injEq]
+          congr
+          rw [ih (fun i => P i.succ) ⟨i, h⟩]
+      else
+        simp only [decodeSubtype, dif_neg h₀]
+        cases i using Fin.casesZeroSuccOn with
+        | zero => contradiction
+        | succ i =>
+          rw [encodeSubtype_succ_neg h₀]
+          simp only [coe_cast, Subtype.mk.injEq]
+          congr
+          rw [ih (fun i => P i.succ) ⟨i, h⟩]
+
+/-- Get representative for the equivalence class of `x`. -/
+abbrev getRepr (s : Setoid (Fin n)) [DecidableRel s.r] (x : Fin n) : Fin n :=
+  match h : Fin.find? (s.r x) with
+  | some y => y
+  | none => False.elim <| by
+    have : Fin.find? (s.r x) |>.isSome := by
+      rw [find?_isSome_iff_exists]
+      exists x
+      exact Setoid.refl x
+    simp [h] at this
+
+@[simp] theorem equiv_getRepr (s : Setoid (Fin n)) [DecidableRel s.r] (x : Fin n) :
+    s.r x (getRepr s x) := by
+  apply find?_prop
+  simp only [getRepr]
+  split
+  · assumption
+  · next h =>
+    have : Fin.find? (s.r x) |>.isSome := by
+      rw [find?_isSome_iff_exists]
+      exists x
+      exact Setoid.refl x
+    simp [h] at this
+
+@[simp] theorem getRepr_equiv (s : Setoid (Fin n)) [DecidableRel s.r] (x : Fin n) :
+    s.r (getRepr s x) x := Setoid.symm (equiv_getRepr ..)
+
+theorem getRepr_eq_getRepr_of_equiv (s : Setoid (Fin n)) [DecidableRel s.r] (h : s.r x y) :
+    getRepr s x = getRepr s y := by
+  have hfind : Fin.find? (s.r x) = Fin.find? (s.r y) := by
+    congr
+    funext z
+    apply propext
+    constructor
+    · exact Setoid.trans (Setoid.symm h)
+    · exact Setoid.trans h
+  simp only [getRepr]
+  split
+  · next hx =>
+    rw [hfind] at hx
+    split
+    · next hy =>
+      rwa [hx, Option.some_inj] at hy
+    · next hy =>
+      rw [hx] at hy
+      contradiction
+  · next hx =>
+    rw [hfind] at hx
+    split
+    · next hy =>
+      rw [hx] at hy
+      contradiction
+    · rfl
+
+@[simp] theorem getRepr_getRepr (s : Setoid (Fin n)) [DecidableRel s.r] (x : Fin n) :
+    getRepr s (getRepr s x) = getRepr s x := by
+  apply getRepr_eq_getRepr_of_equiv
+  exact getRepr_equiv ..
+
+/-- Encode decidable quotient of a `Fin` type. -/
+def encodeQuotient (s : Setoid (Fin n)) [DecidableRel s.r] (x : Quotient s) :
+    Fin (Fin.count fun i => getRepr s i = i) :=
+  encodeSubtype _ <| Quotient.liftOn x (fun i => ⟨getRepr s i, getRepr_getRepr s i⟩) <| by
+    intro _ _ h
+    simp only [Subtype.mk.injEq]
+    exact getRepr_eq_getRepr_of_equiv s h
+
+/-- Decode decidable quotient of a `Fin ` type. -/
+def decodeQuotient (s : Setoid (Fin n)) [DecidableRel s.r]
+    (i : Fin (Fin.count fun i => getRepr s i = i)) : Quotient s :=
+  Quotient.mk s (decodeSubtype _ i)
+
+@[simp] theorem encodeQuotient_decodeQuotient (s : Setoid (Fin n)) [DecidableRel s.r] (x) :
+    encodeQuotient s (decodeQuotient s x) = x := by
+  simp only [decodeQuotient, encodeQuotient, Quotient.liftOn, Quotient.mk, Quot.liftOn]
+  conv => rhs; rw [← encodeSubtype_decodeSubtype _ x]
+  congr
+  exact (decodeSubtype _ x).property
+
+@[simp] theorem decodeQuotient_encodeQuotient (s : Setoid (Fin n)) [DecidableRel s.r] (x) :
+    decodeQuotient s (encodeQuotient s x) = x := by
+  induction x using Quotient.inductionOn with
+  | _ x =>
+    simp only [decodeQuotient, encodeQuotient, Quotient.liftOn, Quotient.mk, Quot.liftOn]
+    apply Quot.sound
+    simp
